Merge

timing/examples/FreeRTOS/list/vListInsert.v
@@ -28,19 +28,71 @@ End vListInsertTime.
 Module vListInsertAuto := TimingAutomation vListInsertTime.
 Import vListInsertTime vListInsertAuto.
 
+(* https://github.com/FreeRTOS/FreeRTOS-Kernel/blob/main/include/list.h#L147 *)
+Definition xItemValue (mem : addr -> N) (a : addr) : N :=
+    mem Ⓓ[a].
+Definition pxNext (mem : addr -> N) (a : addr) : addr :=
+    mem Ⓓ[4 + a].
+Definition portMAX_DELAY : N :=
+    0 ⊖ 1.
+
+(* Get the nth item of a linked list *)
+Fixpoint linked_list_access (mem : addr -> N) (a : addr) (n : nat) : addr :=
+    match n with
+    | O => a
+    | S n' => linked_list_access mem (pxNext mem a) n'
+    end.
+
 (* Postcondition *)
-Definition time_of_vListInsert (t : trace) (base_mem : addr -> N) (a0 : N) :=
-    True.
+Definition time_of_vListInsert (t : trace) (base_mem : addr -> N) (a0 a1 : N) :=
+    cycle_count_of_trace t =
+        4 + time_mem.
+
+Definition vListInsert_terminates (mem : addr -> N) 
+    (pxList : addr) (pxNewListItem : addr) : Prop :=
+    let xValueOfInsertion := xItemValue mem pxNewListItem in 
+    xValueOfInsertion = portMAX_DELAY \/
+    exists k, 
+      xItemValue mem (linked_list_access mem pxList k) > xValueOfInsertion.
 
 (* Invariants *)
+(*
+     Entrypoint       
+          |           
+          v           
+  Degeneracy Check    
+          |<---------+
+          v          |
+    Return Point     |
+          |          |
+          v          |
++--->Loop Start      |
+|         |          |
+|         v          |
++----Break Check     |
+          |          |
+          v          |
+      Loop End-------+
+*)
 Definition vListInsert_timing_invs (base_mem : addr -> N) (a0 : N) (a1 : N)
     (t:trace) : option Prop :=
 match t with (Addr a, s) :: t' => match a with
+(* Entrypoint *)
 | 0x800023f0 => Some (s V_MEM32 = Ⓜbase_mem /\ s R_A0 = Ⓓa0 /\ s R_A1 = Ⓓa1 /\
+                      vListInsert_terminates base_mem a0 a1 /\
                         cycle_count_of_trace t' = 0)
+(* Degeneracy Check *)
 | 0x800023fc => Some (exists mem, s V_MEM32 = Ⓜmem /\ 
                         s R_A0 = Ⓓa0 /\ s R_A1 = Ⓓa1 /\
+                        vListInsert_terminates mem a0 a1 /\
                         cycle_count_of_trace t' = 4 + time_mem)
+(* Return Point *)
+| 0x80002428 => Some (time_of_vListInsert t base_mem a0 a1)
+(* Loop Start *)
+| 0x8000242c => Some (exists k, cycle_count_of_trace t' = 
+                        4 + time_mem + time_branch + 
+                        k * (2 + 2 * time_mem + time_branch)
+                     )
 | _ => None end | _ => None end.
 
 (* Lift the program *)
@@ -53,7 +105,8 @@ Theorem vListInsert_timing:
          (MDL: models rvtypctx s)
          (MEM: s V_MEM32 = Ⓜbase_mem)
          (A0: s R_A0 = Ⓓa0)
-         (A1: s R_A1 = Ⓓa1),
+         (A1: s R_A1 = Ⓓa1)
+         (TERMINATES: vListInsert_terminates base_mem a0 a1),
   satisfies_all 
     lifted_vListInsert
     (vListInsert_timing_invs base_mem a0 a1)
@@ -78,9 +131,32 @@ Proof using.
     destruct_inv 32 PRE.
 
     (* Entrypoint *)
-    destruct PRE as (MEM & A0 & A1 & Cycles).
+    destruct PRE as (MEM & A0 & A1 & TERMINATES & Cycles).
     repeat step.
-    (* 0x800023fc *)
-    handle_ex. hammer. find_rewrites. unfold time_mem. lia.
-Admitted.
+    (* 0x800023fc *) {
+        handle_ex. hammer. find_rewrites. unfold time_mem. lia.
+    }
+
+    destruct PRE as (mem & MEM & A0 & A1 & TERMINATES & Cycles).
+    step.
+    (* 0x8000242c - loop entry *) {
+        exists 0. hammer. find_rewrites. unfold time_mem, time_branch.
+        lia.
+    }
+
+    (* 0x80002428 - postcondition after degeneracy check fails *)
+    admit.
+
+    (* 0x8000242c - loop iterate *)
+    repeat step.
+
+    (* 0x80002428 - postcondition after loop exits *)
+    admit.
+
+    (* 0x8000242c - loop invariant after iteration *)
+    destruct PRE as (k & Cycles).
+    exists k. hammer. find_rewrites. apply Bool.negb_true_iff in BC.
+    rewrite BC. psimpl. unfold time_mem, time_branch. psimpl. 
+
+Qed.
 
